Hax.lean
@@ -1,3 +1,4 @@
 import Hax.MissingLean
 import Hax.MissingAeneas
 import Hax.Tactic
+import Hax.Tactic.ForLoopWithInvariantSpec
